Progress with sem pres

src/A/Syntax.v
@@ -1,22 +1,6 @@
 From CoreErlang.Subst Require Export Semantics CIU.
 From stdpp Require Export base list.
 
-
-(* Program contexts for the context-based ANF normalizer.  Unlike the
-   continuation-based normalizer above, the remaining computation is
-   represented explicitly by an [NCtx] frame stack. *)
-Inductive NCtx : Set :=
-| NCHole
-| NCLet (e2 : Exp) (k : NCtx)
-(* | NCCase (p : Pat) (e1 e2 : Exp) (k1 k2 : NCtx) *)
-| NCCase (p : Pat) (e1 e2 : Exp) (k : NCtx)
-| NCApp1 (args : list Exp) (k : NCtx)
-| NCApp2 (f : Val) (done : list Val) (todo : list Exp) (k : NCtx)
-| NCBIF1 (args : list Exp) (k : NCtx)
-| NCBIF2 (f : Val) (done : list Val) (todo : list Exp) (k : NCtx)
-| NCCons1 (e1 : Exp) (k : NCtx)
-| NCCons2 (e2 : Val) (k : NCtx).
-
 Inductive ANF : Exp -> Prop :=
 | anf_val (v : Val) :
   ANF (˝v)
@@ -44,14 +28,12 @@ Inductive ANF : Exp -> Prop :=
   ANF (°ELet (°EBIF v (map VVal vl)) e2)
 .
 
-Definition plug_fs (Fs : FrameStack) (e : Exp) := fold_right plug_f e Fs.
-
 Definition rename_frame (ρ : Renaming) (f : Frame) : Frame :=
 match f with
  | FApp1 l => FApp1 (map (rename ρ) l)
  | FApp2 v l1 l2 => FApp2 (rename_val ρ v) (map (rename_val ρ) l1) (map (rename ρ) l2)
- | FLet e2 => FLet (rename ρ e2)
- | FCase p e2 e3 => FCase p (rename ρ e2) (rename ρ e3)
+ | FLet e2 => FLet (rename (upren ρ) e2)
+ | FCase p e2 e3 => FCase p (rename (uprenn (pat_vars p) ρ) e2) (rename ρ e3)
  | FCons1 e1 => FCons1 (rename ρ e1)
  | FCons2 v2 => FCons2 (rename_val ρ v2)
  | FBIF1 l => FBIF1 (map (rename ρ) l)
@@ -74,354 +56,11 @@ match l with
 | x::xs => if f x then drop_while f xs else xs
 end.
 
-
-Fixpoint split_list_val (l : list Exp) : list Val * list Exp :=
-match l with
-| []    => ([], [])
-| e::es => match e with
-           | VVal v =>
-             let '(vals, exps) := split_list_val es in
-               (v :: vals, exps)
-           | EExp e => ([], EExp e::es)
-           end
-end.
-
 Definition is_value (e : Exp) : bool :=
 match e with
  | EExp e => false
  | VVal v => true
 end.
-
-Definition is_comp_value (e : Exp) : bool :=
-match e with
- | EExp e =>
-   match e with
-    | EBIF exp l | EApp exp l => is_value exp && forallb is_value l
-    | _ => false
-   end   
- | VVal v => true
-end.
-
-(* Takewhile needed *)
-Definition A_normalize_heat (e : Exp) : option (Frame * Exp) :=
-match e with
- | EExp e =>
-   match e with
-   | EApp exp l =>
-     match exp with
-     | VVal v1 =>
-       let '(vals, exps) := split_list_val l in
-         match exps with
-         | [] => None
-         | e::es => Some (FApp2 v1 vals es, e)
-         end
-     | _ => Some (FApp1 l, exp)
-     end
-   | ELet e1 e2 =>
-     if is_comp_value e1
-     then None
-     else Some (FLet e2, e1)
-   | ECase e p e1 e2 =>
-     if is_value e
-     then None
-     else Some (FCase p e1 e2, e)
-   | ECons e1 e2 =>
-     match e2 with
-     | VVal v2 => match e1 with
-                  | VVal v1 => None
-                  | _       => Some (FCons2 v2, e1)
-                  end
-     | _       => Some (FCons1 e1, e2)
-     end
-   | EReceive l => None
-   | EBIF exp l =>
-     match exp with
-     | VVal v1 =>
-       let '(vals, exps) := split_list_val l in
-         match exps with
-         | [] => None
-         | e::es => Some (FBIF2 v1 vals es, e)
-         end
-     | _       => Some (FBIF1 l, exp)
-     end
-  end
- | VVal v => None
-end.
-
-(*
-Full def, but ill-formed due to split:
-
-Fixpoint A_normalize_heat (ebase : Exp) : option (FrameStack * Exp) :=
-match ebase with
- | EExp ee =>
-   match ee with
-   | EApp exp l =>
-     match exp with
-     | VVal v1 =>
-       let '(vals, exps) := split_list_val l in
-         match exps with
-         | [] => None
-         | e::es =>
-            match A_normalize_heat e with
-            | None => Some ([FApp2 v1 vals es], e)
-            | Some (fs, e') => Some (FApp2 v1 vals es :: fs, e')
-            end
-         end
-     | _       => 
-       match A_normalize_heat exp with
-        | None => Some ([FApp1 l], exp)
-        | Some (fs, e') => Some (FApp1 l :: fs, e')
-       end
-     end
-   | ELet e1 e2 =>
-     if is_value e1
-     then None
-     else match A_normalize_heat e1 with
-           | None => Some ([FLet e2], e1)
-           | Some (fs, e') => Some (FLet e2 :: fs, e')
-          end
-   | ECase e p e1 e2 =>
-     if is_value e
-     then None
-     else match A_normalize_heat e with
-           | None => Some ([FCase p e1 e2], e)
-           | Some (fs, e') => Some (FCase p e1 e2 :: fs, e')
-          end
-   | ECons e1 e2 =>
-     match e2 with
-     | VVal v2 => match e1 with
-                  | VVal v1 => None
-                  | _       =>
-                    match A_normalize_heat e1 with
-                     | None => Some ([FCons2 v2], e1)
-                     | Some (fs, e') => Some (FCons2 v2 :: fs, e')
-                    end
-                  end
-     | _       => match A_normalize_heat e1 with
-                   | None => Some ([FCons1 e1], e2)
-                   | Some (fs, e') => Some (FCons1 e1 :: fs, e')
-                  end
-     end
-   | EReceive l => None
-   | EBIF exp l =>
-     match exp with
-     | VVal v1 =>
-       let '(vals, exps) := split_list_val l in
-         match exps with
-         | [] => None
-         | e::es =>
-            match A_normalize_heat e with
-            | None => Some ([FBIF2 v1 vals es], e)
-            | Some (fs, e') => Some (FBIF2 v1 vals es :: fs, e')
-            end
-         end
-     | _       => 
-       match A_normalize_heat exp with
-        | None => Some ([FBIF1 l], exp)
-        | Some (fs, e') => Some (FBIF1 l :: fs, e')
-       end
-     end
-  end
- | VVal v => None
-end.
-*)
-
-Fixpoint A_normalize_heat_rec (iters : nat) (e : Exp) : option (FrameStack * Exp) :=
-match iters with
-| 0 => None
-| S iters' =>
-  match A_normalize_heat e with
-  | None => Some ([], e)
-  | Some (F, e') =>
-    match A_normalize_heat_rec iters' e' with
-    | None => None
-    | Some (Fs, e'') => Some (F::Fs, e'')
-    end
-  end
-end.
-(* TODO: normalize_heat_rec always correctly terminates - see commented def,
-   which would be correct, if we inlined split.
- *)
-
-
-(* TODO: side conds - renamings
-   IN the nameless presentation, the scope order gets reversed by this
-   transformation - therefore, renamings have to be applied to ensure the
-   correct binding structure *)
-Definition A_normalize_reduce (Fs : FrameStack) (e : Exp) : option Exp :=
-match e with
- | EExp (ELet e1 e2) =>
-   (* e2 should not be touched, because it is placed in a position where
-      a closed expression is expected -> we "close it" by the "outer" let
-      Fs does not need to be touched because it is closed -> bindings 
-      cannot get tangled up *)
-   Some (°ELet e1 (plug_fs Fs e2))
- | EExp (ECase e p e1 e2) =>
-   if is_value e
-   (* The same applies here *)
-   then Some (°ECase e p (plug_fs Fs e1) (plug_fs Fs e2))
-   else None
- (* We do not need renaming in the following cases either because
-    we expect that the frame stack is closed, therefore, it does
-    not contain a dangling 0 index, so we can safely put it inside
-    with an outer "let" binding it *)
- | EExp (EApp exp l) =>
-   if is_value exp then if forallb is_value l
-   then Some (°ELet e (plug_fs Fs (VVar 0)))
-   else None
-   else None
- | EExp (EBIF exp l) =>
-   if is_value exp then if forallb is_value l
-   then Some (°ELet e (plug_fs Fs (VVar 0)))
-   else None
-   else None
- | EExp (ECons e1 e2) =>
-   if is_value e1 then if is_value e2
-   then Some (°ELet e (plug_fs Fs (VVar 0)))
-   else None
-   else None
- | _ => None
-end.
-
-(* Better question: normalize heat + normalize reduce repeatedly iterated is OK? *)
-
-Definition A_normalize_step (iters : nat) (e : Exp) : option Exp :=
-  match A_normalize_heat_rec iters e with
-  | Some ([], e) => None
-  | Some (fs, e) => A_normalize_reduce fs e
-  | None => None
-  end.
-
-Fixpoint A_normalize (iters : nat) (iters2 : nat) (e : Exp) : option Exp :=
-match iters with
-| 0 => None
-| S iters' =>
-  match (A_normalize_step iters2 e) with
-  | Some exp => A_normalize iters' iters2 exp
-  | None => Some e (* not OK, if iters2 is too low *)
-  end
-end.
-
-
-Open Scope string_scope.
-Definition ex1 : NonVal :=
-  ELet (VLit 0%Z) (EBIF (VLit "+"%string) [˝VLit 3%Z; ˝VVar 0]).
-Definition fs1 : FrameStack := [FLet (VVar 0)].
-
-Compute plug_fs fs1 ex1.
-Compute A_normalize_reduce fs1 ex1.
-
-
-Compute A_normalize_heat_rec 100 (plug_fs fs1 ex1).
-Compute A_normalize_reduce [(FLet (˝ VVar 0))] (ELet (VLit 0%Z)
-               (EBIF (˝VLit "+")
-                  (cons (˝VLit 3%Z) (cons (˝VVar 0) nil)))).
-
-Compute A_normalize_heat_rec 100 (ELet (VLit 0%Z)
-            (ELet
-               (EBIF (VLit "+")
-                  (cons (˝VLit 3%Z) (cons (˝VVar 0) nil)))
-               (VVar 0))).
-
-Compute A_normalize 100 100 (plug_fs fs1 ex1).
-
-
-
-
-
-
-
-
-
-
-
-
-
-(* Reserved Notation "⟨ Fs , e ⟩ '-A->' ⟨ Fs' , e' ⟩" (at level 60).
-Inductive A_normalize : FrameStack -> Exp -> Exp -> Prop :=
-
-(* actual rules *)
-| norm_let :
-  ⟨Fs, ELet e1 e2⟩ -A-> 
-
-(* construct evaluation context *)
-
-where "⟨ Fs , e ⟩ '-A->' e'" := (A_normalize Fs e e'). *)
-
-(* Inductive Conf : Set :=
-| ELet  (e1 : Comp) (e2 : Conf)
-| ECase (e : Val) (p : Pat) (e1 e2 : Conf)
-| EComp (n : Comp)
-
-with Comp : Set :=
-| EApp (v : Val) (l : list Val)
-| EBIF (v : Val) (l : list Val)
-| EVal (v : Val)
-
-with Val : Set :=
-| VLit   (l : Lit)
-| VVar   (n : nat)
-| VNil
-| VCons (v1 v2 : Val)
-| VClos (Γ : list Val) (vl : nat) (e : Conf). *)
-
-
-(* Inductive NCtx : Set :=
-| CBox
-| CLet (e2 : Exp)
-| CCase (p : Pat) (e1 e2 : Exp)
-| CCons (c1 c2 : NCtx)
-| CApp (c : NCtx) (l : list NCtx)
-| CBIF (c : NCtx) (l : list NCtx).
-
-
-Axiom applyCtx : NCtx -> Exp -> Exp.
-Axiom applyCCtx : NCtx -> NCtx -> NCtx.
-
-Definition normalize_name (f : NCtx -> Exp) (k : NCtx) : Exp. Admitted.
-  (* f (fun e' => if is_value e' then applyCtx k e' else ELet e' (applyCtx k (VVar 0))). *)
-
-Fixpoint normalize (e : Exp) (k : NCtx) {struct e} : Exp :=
-match e with
-| VVal (VFun vl e) => applyCtx k (VVal (VFun vl (normalize e id)))
-| VVal (VCons e1 e2) => applyCtx k e (* TODO: might be wrong *)
-| VVal v => applyCtx k (VVal v)
-| EExp (ELet e1 e2) => normalize e1 (CLet1 (normalize e2 k))
-| EExp (ECase e p e1 e2) => normalize_name (normalize e) (applyCCtx k (CCase1 p (normalize e1 k) (normalize e2 k)))
-| EExp (EApp e1 l) => normalize_name (normalize e1) (fun e1' =>
-     (fix normalize_name_star (l : list Exp) (k : NCtx) {struct l} : Exp :=
-      match l with
-      | [] => k []
-      | e::es => normalize_name (normalize e) (fun e' => normalize_name_star es (fun es' => k (e'::es')))
-      end) l (fun '(l1', l2') => applyCCtx k (CApp2 e1' l1' l2')))
-| EExp (EBIF e1 l) => normalize_name (normalize e1) (fun e1' => 
-     (fix normalize_name_star (l : list Exp) (k : NCtx) {struct l} : Exp :=
-      match l with
-      | [] => k []
-      | e::es => normalize_name (normalize e) (fun e' => normalize_name_star es (fun es' => k (e'::es')))
-      end) l (fun '(l1', l2') => applyCCtx k (CBIF2 e1' l1' l2')))
-| EExp (ECons e1 e2) => normalize_name (normalize e2) (applyCCtx k (CCons CBox CBox))
-
-normalize_name (normalize e2)
-  (fun e2' => normalize_name (normalize e1) (fun e1' => k (ECons e1' e2')))
-
-
-
-
-(fun e2' => normalize_name (normalize e1) (fun e1' => applyCCtx k (CCons1 e1')))
-| EExp (EReceive l) => inf (* TODO option? *)
-end.
-
-Definition normalize_term (e : Exp) : Exp := normalize e id. *)
-
-
-
-
-
-
-
-
-
 
 Definition normalize_name (f : (Exp -> Exp) -> Exp) (k : Exp -> Exp) : Exp :=
   f (fun e' => if is_value e' then k e' else ELet e' (k (VVar 0))).
@@ -451,28 +90,6 @@ end.
 
 Definition normalize_term (e : Exp) : Exp := normalize e id.
 
-Fixpoint rename_nctx (ρ : Renaming) (k : NCtx) : NCtx :=
-  match k with
-  | NCHole => NCHole
-  | NCLet e2 k' =>
-      NCLet (rename (upren ρ) e2) (rename_nctx (upren ρ) k')
-  (* | NCCase p e1 e2 k1 k2 =>
-      NCCase p (rename (uprenn (pat_vars p) ρ) e1) (rename ρ e2)
-        (rename_nctx (uprenn (pat_vars p) ρ) k1) (rename_nctx ρ k2) *)
-  | NCCase p e1 e2 k =>
-      NCCase p (rename (uprenn (pat_vars p) ρ) e1) (rename ρ e2) (rename_nctx ρ k)
-  | NCApp1 args k' => NCApp1 (map (rename ρ) args) (rename_nctx ρ k')
-  | NCApp2 f done todo k' =>
-      NCApp2 (rename_val ρ f) (map (rename_val ρ) done) (map (rename ρ) todo)
-        (rename_nctx ρ k')
-  | NCBIF1 args k' => NCBIF1 (map (rename ρ) args) (rename_nctx ρ k')
-  | NCBIF2 f done todo k' =>
-      NCBIF2 (rename_val ρ f) (map (rename_val ρ) done) (map (rename ρ) todo)
-        (rename_nctx ρ k')
-  | NCCons1 e1 k' => NCCons1 (rename ρ e1) (rename_nctx ρ k')
-  | NCCons2 e2 k' => NCCons2 (rename_val ρ e2) (rename_nctx ρ k')
-  end.
-
 Definition introduce_let  (normalize_exp : Exp -> FrameStack -> option Exp) 
                           (k : FrameStack) (e : Exp) : option Exp :=
 match k with
@@ -494,13 +111,13 @@ Fixpoint normalize_exp (fuel : nat) (e : Exp) (k : FrameStack) : option Exp :=
           mbind (fun body' =>
           normalize_val fuel' (VFun vl body') k)
           (normalize_exp fuel' body [])
-        | VVal v => normalize_val fuel' v k
-        | EExp (ELet e1 e2) => normalize_exp fuel' e1 (FLet e2 :: k)
+      | VVal v => normalize_val fuel' v k
+      | EExp (ELet e1 e2) => normalize_exp fuel' e1 (FLet e2 :: k)
       | EExp (ECase e0 p e1 e2) =>
           normalize_exp fuel' e0 (FCase p e1 e2 :: k)
-        | EExp (EApp f args) => normalize_exp fuel' f (FApp1 args :: k)
-        | EExp (EBIF f args) => normalize_exp fuel' f (FBIF1 args :: k)
-        | EExp (ECons e1 e2) => normalize_exp fuel' e2 (FCons1 e1 :: k)
+      | EExp (EApp f args) => normalize_exp fuel' f (FApp1 args :: k)
+      | EExp (EBIF f args) => normalize_exp fuel' f (FBIF1 args :: k)
+      | EExp (ECons e1 e2) => normalize_exp fuel' e2 (FCons1 e1 :: k)
       | EExp (EReceive cases) => None
       (*  continue_ctx_fuel fuel' k (EReceive cases) *)
       end
@@ -612,30 +229,6 @@ Definition anf_examples : list (Exp * Exp) :=
   ; (anf_case_branch_src, anf_case_branch_anf)
   ].
 
-(* Compute A_normalize_heat_compatible anf_bif_args_src.
-Compute A_normalize_reduce ([AHeatEval (FBIF2 (VLit "+") []
-              [° (EBIF (VLit "+") [˝VLit 3%Z; ˝VLit 4%Z])])])
-              (EBIF (VLit "+") [˝VLit 1%Z; ˝VLit 2%Z]).
-Compute A_normalize_heat_compatible (° ELet
-(° EBIF (˝ VLit "+") [˝ VLit 1%Z;
-˝ VLit 2%Z])
-(° EBIF (˝ VLit "+")
-[˝ VVar 0;
-° EBIF (˝ VLit "+")
-[˝ VLit 3%Z; ˝ VLit 4%Z]])).
-Compute A_normalize_reduce [AHeatLetBody
-(° EBIF (˝ VLit "+") [˝ VLit 1%Z; ˝ VLit
-2%Z]);
-AHeatEval (FBIF2 (VLit "+") [VVar 0] [])] (° EBIF (˝ VLit "+") [˝ VLit 3%Z; ˝ VLit 4%Z]).
-Compute A_normalize_heat_compatible (° ELet
-(° EBIF (˝ VLit "+") [˝ VLit 3%Z;
-˝ VLit 4%Z])
-(° ELet
-(° EBIF (˝ VLit "+")
-[˝ VLit 1%Z; ˝ VLit 2%Z])
-(° EBIF (˝ VLit "+")
-[˝ VVar 0; ˝ VVar 0]))). *)
-
 Notation "'let' e1 'in' e2" := (ELet e1 e2) (only printing, at level 70, e2 at level 10).
 Notation "'call' e1 ( e2 ; e3 ; .. ; en )" := (EBIF e1 (cons e2 (cons e3 .. (cons en nil) .. )) ) (only printing, at level 70).
 
@@ -674,14 +267,6 @@ Qed.
 End Examples.
 
 
-
-
-
-
-
-
-
-
 Fixpoint size_exp (e : Exp) : nat :=
   match e with
   | EExp ne =>
@@ -708,59 +293,48 @@ with size_val (v : Val) : nat := (* technical *)
   | VCons v1 v2 => S (size_val v1 + size_val v2)
   end.
 
-Fixpoint size_nctx (k : NCtx) : nat :=
-  match k with
-  | NCHole => 0
-  | NCLet e2 k' => (size_exp e2 + size_nctx k')
-  | NCCase _ e1 e2 k' => (size_exp e1 + size_exp e2 + size_nctx k')
-  | NCApp1 args k' =>
-    (foldr (fun x acc => size_exp x + acc) 0 args + size_nctx k')
-  | NCApp2 f done todo k' =>
-    (* S (size_exp f + *)
-      (* foldr (fun x acc => size_exp x + acc) 0 done + *)
-      foldr (fun x acc => size_exp x + acc) 0 todo + size_nctx k'
-  | NCBIF1 args k' =>
-    (foldr (fun x acc => size_exp x + acc) 0 args + size_nctx k')
-  | NCBIF2 f done todo k' =>
-    (* S (size_exp f + *)
-      (* foldr (fun x acc => size_exp x + acc) 0 done + *)
-      foldr (fun x acc => size_exp x + acc) 0 todo + size_nctx k'
-  | NCCons1 e1 k' => (size_exp e1 + size_nctx k')
-  | NCCons2 e2 k' => ( (*size_exp e2 +*) size_nctx k')
-  end.
+Lemma Private_size_rename :
+  (forall e ρ, size_exp (rename ρ e) = size_exp e) /\
+  (forall e ρ, size_exp (rename_nonval ρ e) = size_exp e) /\
+  (forall e ρ, size_val (rename_val ρ e) = size_val e).
+Proof.
+  apply Exp_full_ind with
+    (Q := Forall (fun e => forall ρ, size_exp (rename ρ e) = size_exp e))
+    (W := Forall (fun '(_, e) => forall ρ, size_exp (rename ρ e) = size_exp e))
+  ; simpl; intros; try lia.
+  * by rewrite H.
+  * rewrite H. lia.
+  * rewrite H. lia.
+  * rewrite H. f_equal. f_equal.
+    induction H0; simpl. lia.
+    rewrite H0. f_equal. assumption.
+  * rewrite H, H0. lia.
+  * rewrite H, H0, H1. lia.
+  * rewrite H, H0. lia.
+  * rewrite H, H0. lia.
+  * rewrite H. f_equal. f_equal.
+    induction H0; simpl. lia.
+    rewrite H0. f_equal. assumption.
+  * f_equal.
+    induction H; simpl. lia. destruct x.
+    rewrite H. f_equal. assumption.
+  * constructor.
+  * by constructor.
+  * constructor.
+  * by constructor.
+Qed.
 
+Lemma size_rename :
+  (forall e ρ, size_exp (rename ρ e) = size_exp e).
+Proof.
+  apply Private_size_rename.
+Qed.
 
-Lemma size_rename_exp :
-  forall e ρ, size_exp (rename ρ e) = size_exp e.
-Proof. Check Exp_ind2.
-  (* refine
-    (Exp_ind2
-       (P := fun e => forall ρ, size_exp (rename ρ e) = size_exp e)
-       (PV := fun v => forall ρ, size_val (rename_val ρ v) = size_val v)
-       (PN := fun nv => forall ρ, size_exp (EExp (rename_nonval ρ nv)) = size_exp (EExp nv))
-       (Q := fun l =>
-               forall ρ,
-                 foldr (fun x acc => size_exp x + acc) 0 (map (rename ρ) l) =
-                 foldr (fun x acc => size_exp x + acc) 0 l)
-       (W := fun l =>
-               forall ρ,
-                 foldr (fun '(p, e) acc => size_exp e + acc) 0
-                   (map (fun '(p, v) => (p, rename (uprenn (pat_vars p) ρ) v)) l) =
-                 foldr (fun '(p, e) acc => size_exp e + acc) 0 l));
-    cbn; intros; try reflexivity.
-  - intros ρ. now rewrite H.
-  - intros ρ. exact (H ρ).
-  - intros ρ. now rewrite H.
-  - intros ρ. now rewrite H, H0.
-  - intros ρ. now rewrite H, H0, H1.
-  - intros ρ. now rewrite H, H0.
-  - intros ρ. now rewrite H, H0.
-  - intros ρ. now rewrite H.
-  - intros ρ. now rewrite H, H0.
-  - intros ρ. now rewrite H, H0.
-  - intros ρ. now rewrite H, H0.
-  - intros ρ. now rewrite H, H0. *)
-Admitted.
+Lemma size_rename_val :
+  (forall e ρ, size_val (rename_val ρ e) = size_val e).
+Proof.
+  apply Private_size_rename.
+Qed.
 
 Lemma fold_size_exp_rename :
   forall ρ l,
@@ -769,124 +343,9 @@ Lemma fold_size_exp_rename :
 Proof.
   intros ρ l.
   induction l as [|x xs IH]; cbn; [reflexivity|].
-  now rewrite size_rename_exp, IH.
+  now rewrite size_rename, IH.
 Qed.
 
-Lemma size_nctx_rename_nctx :
-  forall ρ k, size_nctx (rename_nctx ρ k) = size_nctx k.
-Proof.
-  (* intros ρ k.
-  induction k as
-    [
-    | e2 k' IH
-    | p e1 e2 k' IH
-    | args k' IH
-    | f done todo k' IH
-    | args k' IH
-    | f done todo k' IH
-    | e1 k' IH
-    | e2 k' IH
-    ]; cbn.
-  - reflexivity.
-  - now rewrite size_exp_rename, IH.
-  - now rewrite size_exp_rename, size_exp_rename, IH.
-  - now rewrite fold_size_exp_rename, IH.
-  - now rewrite fold_size_exp_rename, IH.
-  - now rewrite fold_size_exp_rename, IH.
-  - now rewrite fold_size_exp_rename, IH.
-  - now rewrite size_exp_rename, IH.
-  - exact IH. *)
-Admitted.
-
-(* Lemma normalize_total_helper :
-    (forall (e : Exp) k, exists fuel, normalize_exp fuel e k <> None) /\
-    (forall (e : NonVal) k, exists fuel, normalize_exp fuel e k <> None) /\
-    (forall (e : Val) k, exists fuel, normalize_val fuel e k <> None).
-Proof.
-  apply Exp_full_ind with
-      (Q := Forall (fun e => forall k, exists fuel, normalize_exp fuel e k <> None))
-      (W := Forall (fun '(_, e) => forall k, exists fuel, normalize_exp fuel e k <> None)); intros.
-
-
-Admitted. *)
-Print NCtx.
-(* Inductive preANF : NCtx -> Prop :=
-| preANF_hole :
-  preANF NCHole
-
-| preANF_let e1 k:
-  preANF k
-->
-  preANF (NCLet e1 k)
-
-| preANF_case p e1 e2 k:
-  preANF k
-->
-  preANF (NCCase p e1 e2 k)
-
-| preANF_app1 l k:
-  preANF k
-->
-  preANF (NCApp1 l k)
-
-| preANF_bif1 l k:
-  preANF k
-->
-  preANF (NCBIF1 l k)
-
-| preANF_app2 f done todo k:
-  Forall ANF done -> ANF f -> preANF k
-->
-  preANF (NCApp2 f done todo k)
-
-| preANF_bif2 f done todo k:
-  Forall ANF done -> ANF f -> preANF k
-->
-  preANF (NCBIF2 f done todo k)
-
-| preANF_cons1 e1 k:
-  preANF k
-->
-  preANF (NCCons1 e1 k)
-
-| preANF_cons2 e2 k:
-  ANF e2 -> preANF k
-->
-  preANF (NCCons2 e2 k). *)
-
-(* Lemma rename_ANF :
-  forall e ρ, ANF e -> ANF (rename ρ e).
-Proof.
-
-Admitted. *)
-
-(* Lemma rename_preANF :
-  forall k ρ, preANF k -> preANF (rename_nctx ρ k).
-Proof.
-
-Admitted. *)
-
-(* Lemma Private_introduce_let_ANF k e anf fuel :
-  (forall e k anf, preANF k ->
-    normalize_exp fuel e k = Some anf -> ANF anf) ->
-  preANF k -> ANF e -> introduce_let (normalize_exp fuel) k e = Some anf ->
-  ANF anf.
-Proof.
-  intros * IH Hpre He H.
-  unfold introduce_let in H.
-  destruct k; inv Hpre.
-  * assumption.
-  * destruct normalize_exp eqn:Hexp in H; simpl in H; inv H.
-    apply IH in Hexp. 2: assumption.
-    
-  *
-  *
-  *
-  *
-  *
-  *
-  *
-Qed. *)
 
 Lemma normalize_is_ANF :
   forall fuel e k anf, (* preANF k -> *)
@@ -1227,234 +686,4 @@ Proof.
                 apply IHfuel in Hexp; [ by rewrite <- map_app with (l' := [VCons v1 v2]); apply anf_let_bif |lia].
         ** apply IHfuel in H; [assumption | lia ].
 Qed.
-
-(* NOTE:
-   This version won't hold, even though, it shows promising progress. The issue
-   is with i) scoping and ii) closures.
-
-   i) introduce_let is used inside a let expression, and therefore, the scope
-      of the normalisation is 1 + (the scope of the original expression). This
-      scope extension is not expressed in the statement.
-   ii) the syntax of closures get altered---the closure body is adjusted to be
-      in ANF form. Therefore, the final results (if they are closures) could
-      not be proven equal. This could be avoided by the use of CIU.
-
- *)
-Lemma normalize_preserves_semantics fuel : forall k e anf v,
-  ⟨k, e⟩ -->* v ->
-  normalize_exp fuel e k = Some anf ->
-  ⟨[], anf⟩ -->* v.
-Proof.
-Abort.
-(*   induction fuel using lt_wf_ind. rename H into IHfuel.
-  destruct fuel; intros * (* Hpre *) D H; simpl in H. congruence.
-  destruct e; simpl in H; try congruence.
-  * destruct e; simpl in H; try congruence.
-    - eapply IHfuel in H. eassumption. lia.
-      inv D. inv H0. inv H1.
-      by eexists.
-    - eapply IHfuel in H. eassumption. lia.
-      inv D. inv H0. inv H1.
-      by eexists.
-    - eapply IHfuel in H. eassumption. lia.
-      inv D. inv H0. inv H1.
-      by eexists.
-    - eapply IHfuel in H. eassumption. lia.
-      inv D. inv H0. inv H1.
-      by eexists.
-    - eapply IHfuel in H. eassumption. lia.
-      inv D. inv H0. inv H1.
-      by eexists.
-  * destruct v0; simpl in H; try congruence.
-    (* The following technique is repeated for almost all values: ("-" bullets) *)
-    - destruct fuel; simpl in *; try congruence.
-      destruct k; simpl in *. 2: destruct f.
-      + inv H. assumption.
-      + destruct l0.
-        ** unfold introduce_let in H.
-           destruct k.
-           1: { inv H. inv D. eexists. econstructor. constructor. eassumption. }
-           destruct f; simpl in *.
-           all: destruct normalize_exp eqn:Hexp in H; simpl in H.
-           
-           
-            inv H.
-           -- destruct fuel; simpl in *; try congruence.
-              destruct fuel; simpl in *; try congruence.
-        ** eapply IHfuel in H. eassumption. lia.
-           inv D. inv H0. inv H1.
-           by eexists.
-      +
-      +
-      +
-      +
-      +
-      +
-      +
-    -
-    -
-    -
-    -
-    - *)
-Qed.
-
-
-
-
-
-
-
-
-
-
-
-
-
-
-
-
-
-
-Fixpoint NCtx_to_FrameStack (k : NCtx) : FrameStack :=
-match k with
- | NCHole => []
- | NCLet e2 k => FLet e2 :: NCtx_to_FrameStack k
- | NCCase p e1 e2 k => FCase p e1 e2 :: NCtx_to_FrameStack k
- | NCApp1 args k => FApp1 args :: NCtx_to_FrameStack k
- | NCApp2 f done todo k => FApp2 f done todo :: NCtx_to_FrameStack k
- | NCBIF1 args k => FBIF1 args :: NCtx_to_FrameStack k
- | NCBIF2 f done todo k => FBIF2 f done todo :: NCtx_to_FrameStack k
- | NCCons1 e1 k => FCons1 e1 :: NCtx_to_FrameStack k
- | NCCons2 e2 k => FCons2 e2 :: NCtx_to_FrameStack k
-end.
-
-
-
-  
-
-
-
-
-
-Lemma normalize_total_helper :
-  (forall e k, normalize_exp (size_exp e + 2* size_nctx k) e k <> None).
-Proof.
-  intros.
-  remember (size_exp e + 2* size_nctx k) as fuel.
-  assert (fuel >= size_exp e + 2* size_nctx k) as Hfuel by lia. clear Heqfuel.
-  revert e k Hfuel.
-  induction fuel using lt_wf_ind; intros e k Hfuel.
-  intro. destruct fuel, e; simpl in H0, Hfuel; try lia.
-  * destruct e eqn:P.
-    - eapply H in H0. assumption. lia. simpl. lia.
-    - eapply H in H0. assumption. lia. simpl. lia.
-    - eapply H in H0. assumption. lia. simpl. lia.
-    - eapply H in H0. assumption. lia. simpl. lia.
-    - (* TODO: receive *) admit.
-    - eapply H in H0. assumption. lia. simpl. lia.
-  * destruct v; simpl in *.
-    (* The proofs here should all be the same (except for VClos) *)
-    - destruct fuel; simpl in *; try lia.
-      destruct k; cbn in *; try congruence.
-      + destruct normalize_exp eqn:Hexp; simpl in H0; try congruence.
-        eapply H in Hexp. assumption. lia. simpl. lia.
-      + destruct normalize_exp eqn:Hexp; simpl in H0; try congruence.
-        2: { eapply H in Hexp. assumption. lia. simpl. lia. }
-        destruct (normalize_exp fuel e1) eqn:Hexp2; simpl in H0; try congruence.
-        eapply H in Hexp2. assumption. lia. simpl. lia.
-      + destruct args; simpl in Hfuel.
-        ** unfold introduce_let in H0. destruct k; try congruence.
-        (* The proofs here should all be the repetitive *)
-           -- destruct normalize_exp eqn:Hexp; simpl in H0; try congruence.
-              eapply H in Hexp. assumption. lia. simpl. cbn in Hfuel. lia.
-           -- case_match. by cbn in H1.
-              destruct fuel; simpl in *; try lia.
-              destruct fuel; simpl in *; try lia.
-              destruct (normalize_exp)eqn:Hexp in H0; simpl in H0; try congruence.
-              2: {  eapply H in Hexp. assumption. lia. simpl. cbn in Hfuel. lia. }
-              
-              eapply H in Hexp. assumption. lia. simpl. cbn in Hfuel.
-
-
-              rewrite size_nctx_rename_nctx, size_rename_exp, size_rename_exp. lia.
-           -- case_match. by cbn in H1.
-              destruct normalize_exp eqn:Hexp; simpl in H0; try congruence.
-              eapply H in Hexp. assumption. lia. simpl. cbn in Hfuel.
-              admit.
-           -- case_match. by cbn in H1.
-              destruct normalize_exp eqn:Hexp; simpl in H0; try congruence.
-              eapply H in Hexp. assumption. lia. simpl. cbn in Hfuel.
-              admit.
-           -- case_match. by cbn in H1.
-              destruct normalize_exp eqn:Hexp; simpl in H0; try congruence.
-              eapply H in Hexp. assumption. lia. simpl. cbn in Hfuel.
-              admit.
-           -- case_match. by cbn in H1.
-              destruct normalize_exp eqn:Hexp; simpl in H0; try congruence.
-              eapply H in Hexp. assumption. lia. simpl. cbn in Hfuel.
-              admit.
-           -- case_match. by cbn in H1.
-              destruct normalize_exp eqn:Hexp; simpl in H0; try congruence.
-              eapply H in Hexp. assumption. lia. simpl. cbn in Hfuel.
-              admit.
-           -- case_match. by cbn in H1.
-              destruct normalize_exp eqn:Hexp; simpl in H0; try congruence.
-              eapply H in Hexp. assumption. lia. simpl. cbn in Hfuel.
-              admit.
-        ** destruct normalize_exp eqn:Hexp; simpl in H0; try congruence.
-           eapply H in Hexp. assumption. lia. simpl. lia.
-      + destruct todo; simpl in Hfuel.
-        ** unfold introduce_let in H0. destruct k; try congruence.
-        (* The proofs here should all be the repetitive *)
-           -- destruct normalize_exp eqn:Hexp; simpl in H0; try congruence.
-              eapply H in Hexp. assumption. lia. simpl. cbn in Hfuel. lia.
-           -- case_match. by cbn in H1.
-              destruct normalize_exp eqn:Hexp; simpl in H0; try congruence.
-              eapply H in Hexp. assumption. lia. simpl. cbn in Hfuel.
-              admit.
-           -- case_match. by cbn in H1.
-              destruct normalize_exp eqn:Hexp; simpl in H0; try congruence.
-              eapply H in Hexp. assumption. lia. simpl. cbn in Hfuel.
-              admit.
-           -- case_match. by cbn in H1.
-              destruct normalize_exp eqn:Hexp; simpl in H0; try congruence.
-              eapply H in Hexp. assumption. lia. simpl. cbn in Hfuel.
-              admit.
-           -- case_match. by cbn in H1.
-              destruct normalize_exp eqn:Hexp; simpl in H0; try congruence.
-              eapply H in Hexp. assumption. lia. simpl. cbn in Hfuel.
-              admit.
-           -- case_match. by cbn in H1.
-              destruct normalize_exp eqn:Hexp; simpl in H0; try congruence.
-              eapply H in Hexp. assumption. lia. simpl. cbn in Hfuel.
-              admit.
-           -- case_match. by cbn in H1.
-              destruct normalize_exp eqn:Hexp; simpl in H0; try congruence.
-              eapply H in Hexp. assumption. lia. simpl. cbn in Hfuel.
-              admit.
-           -- case_match. by cbn in H1.
-              destruct normalize_exp eqn:Hexp; simpl in H0; try congruence.
-              eapply H in Hexp. assumption. lia. simpl. cbn in Hfuel.
-              admit.
-        ** destruct normalize_exp eqn:Hexp; simpl in H0; try congruence.
-           eapply H in Hexp. assumption. lia. simpl. lia.
-      (* + 
-      +
-      +
-      +
-    - admit.
-    - admit.
-    - admit.
-    - admit.
-    - admit. *)
-Admitted. *)
-
-(* Corollary normalize_ctx_term_total :
-  forall e, exists limit e', normalize_ctx_term e limit = Some e'.
-Proof.
-  intros e.
-  exact (proj1 normalize_total e NCHole).
-Qed. *)
-
-
 
